# a

```python
sage: (x*(x - 1)*(x -l)).expand()
-l*x^2 + x^3 + l*x - x^2
# ...
sage: ((x - (l + 1)/3)^3).expand() + ((x - (l + 1)/3)*(-1/3*l^2 - 2/3*l - 1/3 + l))
....: expand() + (-2/27*l^3 - 2/9*l^2 - 2/9*l - 2/27 + 1/3*l + 1/3*l^2)
-l*x^2 + x^3 + l*x - x^2
sage: x1 = x - (l + 1)/3
sage: A = (-1/3*l^2 - 2/3*l - 1/3 + l)
sage: B = (-2/27*l^3 - 2/9*l^2 - 2/9*l - 2/27 + 1/3*l + 1/3*l^2)
sage: bool(x1^3 + A*x1 + B == x*(x - 1)*(x - l))
True
```

\begin{align*}
j &= 1728 \frac{4A^3}{4A^3 + 27 B^2} \\
    &= 1728
\end{align*}

```python
sage: bool(2^8 * ((l^2 - l + 1)^3 / (l^2 * (l - 1)^2)) == 1728 * (4*A^3)/(4*A^3 + 2
....: 7 * B^2))
True
```

