# a

$$h(x, y) = (x, -y)$$
$$h(\infty) = \infty$$
$$P = (x_1, y_1), \qquad Q = (x_2, y_2)$$
Computing $P + Q$
$$m = \frac{y_2 - y_1}{x_2 - x_1}$$
$$x_3 = m^3 - x_1 - x_2$$
$$h(P + Q)_y = -m (x_3 - x_1) + y_1$$
Now let $y_2' = - y_2, y_1' = -y_1 \implies m' = -m$
$$\implies [h(P) + h(Q)]_y = h(P + Q)_y$$

# b

$$\phi(x, y) = (\omega_3 x, -y)$$
is automorphism of
$$E: y^2 = x^3 + B$$
$$h : \bar{K} \rightarrow \bar{K}$$
$$h(u) = \omega u$$
$$v \in \bar{K}, u = \omega^{-1} v$$
$$h(u) = h(v) \implies \omega u = \omega v \implies u = v$$
$$\phi(\infty) = \infty$$
$$m = \frac{y_2 - y_1}{x_2 - x_1}, x_3 = m^2 - x_1 - x_2$$
$$\phi(P + Q) = (\omega x_3, -y_3)$$
$$\phi(P) = (\omega x_1, -y_1)$$
$$\phi(Q) = (\omega x_2, -y_2)$$
$$m' = -\frac{1}{\omega}m$$
$$x_3' = \frac{1}{\omega^2}m^2 - \omega x_1 - \omega x_2$$
but $\frac{1}{\omega^2}= \omega^{-2}= \omega$, so $x_3' = \omega x_3$
$$\implies \phi(P + Q) = \phi(P) + \phi(Q)$$

# c

