# a

$K$ is isomorphic to $F_3$ which is an algebraically closed field.

$a_2 \neq 0$ or $a_4 \neq 0$ is the same as saying $a_2 = 0$ and $a_4 = 0$.
In which case $y^2 = x^3 + a_6$, and the curve is singular and not
an elliptic curve.

# b

```python
sage: x = var("x")
sage: f = lambda x1, a2, a6: (x1^3 + a2*x1^2 + a6).collect(x)
sage: a2, a4, a6 = var("a2 a4 a6")
sage: f(x - (a4/a6), a2, a6)
(a2 - 3*a4/a6)*x^2 + x^3 - (2*a2*a4/a6 - 3*a4^2/a6^2)*x + a2*a4^2/a6^2 + a6 - a4^3/a
6^3
sage: y = var("y")
sage: (y == f(x - (a4/a6), 0, a6))
y == x^3 - 3*a4*x^2/a6 + a6 + 3*a4^2*x/a6^2 - a4^3/a6^3
sage: (y == f(x - (a4/a6), +3*a4/a6 + a2, a6))
y == a2*x^2 + x^3 - (2*a2*a4/a6 + 3*a4^2/a6^2)*x + a2*a4^2/a6^2 + a6 + 2*a4^3/a6^3
sage: (y == f(x - (a4/a6), 0, 0))
y == x^3 - 3*a4*x^2/a6 + 3*a4^2*x/a6^2 - a4^3/a6^3
sage: ((y + 3*a4*x)^2).collect(x) == f(x - (a4/a6), +3*a4/a6 + a2, a6))
  Input In [24]
    ((y + Integer(3)*a4*x)**Integer(2)).collect(x) == f(x - (a4/a6), +Integer(3)*a4/
a6 + a2, a6))

            ^
SyntaxError: unmatched ')'

sage: (((y + 3*a4*x)^2).collect(x) == f(x - (a4/a6), +3*a4/a6 + a2, a6))
9*a4^2*x^2 + 6*a4*x*y + y^2 == a2*x^2 + x^3 - (2*a2*a4/a6 + 3*a4^2/a6^2)*x + a2*a4^2
/a6^2 + a6 + 2*a4^3/a6^3
sage: (y == f(x - (a4/a6), 0, 0))
y == x^3 - 3*a4*x^2/a6 + 3*a4^2*x/a6^2 - a4^3/a6^3
sage: (y^2 == f(x - (a4/a6), 0, 0))
y^2 == x^3 - 3*a4*x^2/a6 + 3*a4^2*x/a6^2 - a4^3/a6^3
sage: (y^2 == f(x - (a4/a6), a4*(a2 - 1), 0))
y^2 == (a2*a4 - a4 - 3*a4/a6)*x^2 + x^3 + a2*a4^3/a6^2 - (2*a2*a4^2/a6 - 2*a4^2/a6 -
 3*a4^2/a6^2)*x - a4^3/a6^2 - a4^3/a6^3
sage: (y^2 == f(x - (a4/a6), 0, 0))
y^2 == x^3 - 3*a4*x^2/a6 + 3*a4^2*x/a6^2 - a4^3/a6^3
sage: (y^2 == f(x - (a4/a6), +3*a4, 0))
y^2 == 3*(a4 - a4/a6)*x^2 + x^3 - 3*(2*a4^2/a6 - a4^2/a6^2)*x + 3*a4^3/a6^2 - a4^3/a
6^3
sage: (y^2 == f(x - (a4/a6), +3*a4/a6, 0))
y^2 == x^3 - 3*a4^2*x/a6^2 + 2*a4^3/a6^3
sage: (y^2 == f(x - (a4/a6), 0, 0))
y^2 == x^3 - 3*a4*x^2/a6 + 3*a4^2*x/a6^2 - a4^3/a6^3
sage: (y^2 == f(x - (a4/a6), a2, 0))
y^2 == (a2 - 3*a4/a6)*x^2 + x^3 - (2*a2*a4/a6 - 3*a4^2/a6^2)*x + a2*a4^2/a6^2 - a4^3
/a6^3
sage: (y^2 == f(x - (a4/a6), a2, + a2*a4^2/a6^2 - a4^3
....: /a6^3))
y^2 == (a2 - 3*a4/a6)*x^2 + x^3 - (2*a2*a4/a6 - 3*a4^2/a6^2)*x + 2*a2*a4^2/a6^2 - 2*
a4^3/a6^3
sage: (y^2 == f(x - (a4/a6), a2, + a2*a4^2/a6^2 - a4^3/a6^3))
y^2 == (a2 - 3*a4/a6)*x^2 + x^3 - (2*a2*a4/a6 - 3*a4^2/a6^2)*x + 2*a2*a4^2/a6^2 - 2*
a4^3/a6^3
sage: (y^2 == f(x - (a4/a6), a2, + a4^3/a6^3))
y^2 == (a2 - 3*a4/a6)*x^2 + x^3 - (2*a2*a4/a6 - 3*a4^2/a6^2)*x + a2*a4^2/a6^2
sage: (y^2 == f(x - (a4/a6), a2, + a4^3/a6^3 + a6))
y^2 == (a2 - 3*a4/a6)*x^2 + x^3 - (2*a2*a4/a6 - 3*a4^2/a6^2)*x + a2*a4^2/a6^2 + a6
```

Now note that $a_2 a_4 = 0$ and field is characteristic 3.

```python
sage: y^2 == a2*x^2 + x^3 + a6
```

# c

Note that $a_4, a_4' = 0$, so we get $a_2'^3 / a_6' = a_2^3 / a_6$.
$$u^2 = \frac{a_2'}{a_2}$$
$u \in \bar{K}$ because $u$ is the root of $x^2 - u^2$ and $u^2 \in K$.

# d

just sub in the values and solve for $b, c$.

# e

The map $f(x) = x^p$ defines the frobenius endomorphism which is injective from $K \rightarrow K$.
Therefore $a_2^3 / a_6$ can define all the rational values of $K$.

# f

The generalized elliptic curve formula can be turned into the Weierstrauss form and we can assume
$a_4 = 0$. Otherwise $a_2 = 0$. We can then use either of the facts shown above to transform
one curve into another using the appropriate change of variables.
