```python
sage: t = var("t")
sage: x = -4 + t
sage: y = 6 + mt
---------------------------------------------------------------------------
NameError                                 Traceback (most recent call last)
Input In [3], in <cell line: 1>()
----> 1 y = Integer(6) + mt

NameError: name 'mt' is not defined
sage: m = var("m")
sage: y = 6 + mt
---------------------------------------------------------------------------
NameError                                 Traceback (most recent call last)
Input In [5], in <cell line: 1>()
----> 1 y = Integer(6) + mt

NameError: name 'mt' is not defined
sage: y = 6 + m*t
sage: y^2 = x^3 - 25 * x
  Input In [7]
    y**Integer(2) = x**Integer(3) - Integer(25) * x
    ^
SyntaxError: cannot assign to expression here. Maybe you meant '==' instead of '='?

sage: y^2 == x^3 - 25 * x
(m*t + 6)^2 == (t - 4)^3 - 25*t + 100
sage: e = y^2 == x^3 - 25 * x
sage: e
(m*t + 6)^2 == (t - 4)^3 - 25*t + 100
sage: e.expand()
m^2*t^2 + 12*m*t + 36 == t^3 - 12*t^2 + 23*t + 36
sage: e = e.expand()
sage: e -= 36
sage: e
m^2*t^2 + 12*m*t == t^3 - 12*t^2 + 23*t
sage: e -= (e.rhs())
sage: e
m^2*t^2 - t^3 + 12*m*t + 12*t^2 - 23*t == 0
sage: e(m=23/12)
-t^3 + 2257/144*t^2 == 0
sage: e = e(m=23/12)
sage: e /= t^2
sage: e
-1/144*(144*t^3 - 2257*t^2)/t^2 == 0
sage: e.expand()
-t + 2257/144 == 0
sage: e.expand() += t
  Input In [22]
    e.expand() += t
    ^
SyntaxError: 'function call' is an illegal expression for augmented assignment

sage: e.expand() + t
(2257/144) == t
sage: e = e.expand() + t
sage: e
(2257/144) == t
sage: t
t
sage: t = var("t")
sage: m = var("m")
sage: x = -4 + t
sage: y = 6 + m*t
sage: y^2 == x^3 - 25 * x
(m*t + 6)^2 == (t - 4)^3 - 25*t + 100
sage: e = y^2 == x^3 - 25 * x
sage: e
(m*t + 6)^2 == (t - 4)^3 - 25*t + 100
sage: e.expand()
m^2*t^2 + 12*m*t + 36 == t^3 - 12*t^2 + 23*t + 36
sage: e = e.expand()
sage: e
m^2*t^2 + 12*m*t + 36 == t^3 - 12*t^2 + 23*t + 36
sage: e -= (e.rhs())
sage: e
m^2*t^2 - t^3 + 12*m*t + 12*t^2 - 23*t == 0
sage: e(t=0)
0 == 0
sage: e
m^2*t^2 - t^3 + 12*m*t + 12*t^2 - 23*t == 0
sage: e(m=23/12)
-t^3 + 2257/144*t^2 == 0
sage: e = e(m=23/12)
sage: e
-t^3 + 2257/144*t^2 == 0
sage: e /= t^2
sage: e
-1/144*(144*t^3 - 2257*t^2)/t^2 == 0
sage: e.expand()
-t + 2257/144 == 0
sage: e = e.expand()
sage: e
-t + 2257/144 == 0
sage: e += t
sage: e
(2257/144) == t
sage: e.lhs()
2257/144
sage: e.lhs() - 4
1681/144
sage: y = 6 * (23/12)* 2257/144
sage: y
51911/288
sage: y = 6 + (23/12)* 2257/144
sage: y
62279/1728
```

