```python
sage: x1 = 12 * x + 6
sage: y = var("y")
sage: y1 = 72 * y
sage: e = y1^2 == x1^3 - 36*x1
sage: e
5184*y^2 == 216*(2*x + 1)^3 - 432*x - 216
sage: e /= 5184
sage: e
y^2 == 1/24*(2*x + 1)^3 - 1/12*x - 1/24
sage: e.rhs().simplify()
1/24*(2*x + 1)^3 - 1/12*x - 1/24
sage: e.rhs().expand()
1/3*x^3 + 1/2*x^2 + 1/6*x
sage: f = (x*(x + 1)*(2*x + 1) / 6)
sage: e.rhs() == f
1/24*(2*x + 1)^3 - 1/12*x - 1/24 == 1/6*(2*x + 1)*(x + 1)*x
sage: e.rhs() - f
1/24*(2*x + 1)^3 - 1/6*(2*x + 1)*(x + 1)*x - 1/12*x - 1/24
sage: (e.rhs() - f).simplify()
1/24*(2*x + 1)^3 - 1/6*(2*x + 1)*(x + 1)*x - 1/12*x - 1/24
sage: e.rhs().expand() - f.expand()
0
```

